theories/linking/lang.v
@@ -78,124 +78,90 @@ Section Linking.
 
   Implicit Types X : expr * state → Prop.
 
-  (* TODO: Double-check that angelic and demonic nondeterminism and NB and UB are appropiate *)
   Inductive prim_step_mrel (p : prog) : expr * state → (expr * state → Prop) → Prop :=
-  | Step1S e1 C σ X :
-    (* Internal step of an underlying module. *)
-    (∀ σ1 privσ2,
-       σ = St1 σ1 privσ2 →
-       ¬ (∃ K fn_name arg, mlanguage.is_call e1 fn_name arg K ∧ proj1_prog p !! fn_name = None) →
-       mlanguage.to_val e1 = None →
-       ∃ (X1 : _ → Prop),
-         mlanguage.prim_step (proj1_prog p) (e1, σ1) X1 ∧
-         (∀ e1' σ1',
-            X1 (e1', σ1') →
-            X (LkE (Expr1 e1') C, St1 σ1' privσ2))) →
-
-    (* Stuck module calls bubble up as calls at the level of the linking module.
-       (They may get unstuck then, if they match a function implemented by the
-       other module.) *)
-    (∀ pubσ σ1 privσ2 privσ1 fn_name arg k1,
-       σ = St1 σ1 privσ2 →
-       mlanguage.is_call e1 fn_name arg k1 →
-       proj1_prog p !! fn_name = None →
-       mlanguage.split_state σ1 pubσ privσ1 →
-       X (LkE (ExprCall fn_name arg) (inl k1::C), St pubσ privσ1 privσ2)) →
-
-    (* Producing a value when execution is finished *)
-    (∀ σ1 privσ2 pubσ privσ1 v,
-       σ = St1 σ1 privσ2 →
-       mlanguage.to_val e1 = Some v →
-       (* Splitting the state is angelic, the underlying language can choose a concrete splitting. *)
-       (* If no such splitting exists, we have UB *)
-       mlanguage.split_state σ1 pubσ privσ1 →
-       X (LkE (ExprV v) C, St pubσ privσ1 privσ2)) →
-
-    prim_step_mrel p (LkE (Expr1 e1) C, σ) X
-
-  | Step2S e2 C σ X :
-    (* Internal step of an underlying module. *)
-    (∀ σ2 privσ1,
-       σ = St2 privσ1 σ2 →
-       ¬ (∃ K fn_name arg, mlanguage.is_call e2 fn_name arg K ∧ proj2_prog p !! fn_name = None) →
-       mlanguage.to_val e2 = None →
-       ∃ (X2 : _ → Prop),
-         mlanguage.prim_step (proj2_prog p) (e2, σ2) X2 ∧
-         (∀ e2' σ2',
-            X2 (e2', σ2') →
-            X (LkE (Expr2 e2') C, St2 privσ1 σ2'))) →
-
-    (* Stuck module calls bubble up as calls at the level of the linking module.
-       (They may get unstuck then, if they match a function implemented by the
-       other module.) *)
-    (∀ pubσ σ2 privσ1 privσ2 fn_name arg k2,
-       σ = St2 privσ1 σ2 →
-       mlanguage.is_call e2 fn_name arg k2 →
-       proj2_prog p !! fn_name = None →
-       mlanguage.split_state σ2 pubσ privσ2 →
-       X (LkE (ExprCall fn_name arg) (inr k2::C), St pubσ privσ1 privσ2)) →
-
-    (* Producing a value when execution is finished *)
-    (∀ σ2 privσ1 pubσ privσ2 v,
-       σ = St2 privσ1 σ2 →
-       mlanguage.to_val e2 = Some v →
-       (* Splitting the state is angelic, the underlying language can choose a concrete splitting. *)
-       (* If no such splitting exists, we have UB *)
-       mlanguage.split_state σ2 pubσ privσ2 →
-       X (LkE (ExprV v) C, St pubσ privσ1 privσ2)) →
-
-    prim_step_mrel p (LkE (Expr2 e2) C, σ) X
-
-  (* Entering a function. Change the view of the heap in the process. *)
-  | RunFunction1S σ fn1 args C X :
-    (* Merge state and assert that fn1 is applicable to the arguments *)
-    (* If state can not be merged or fn1 not be applied, we have UB *)
-    (* Note that both e1 and σ1 are unique, the latter by split_state_inj *)
-    (∀ e1 σ1 pubσ privσ1 privσ2,
-        σ = St pubσ privσ1 privσ2 →
-        mlanguage.apply_func fn1 args = Some e1 →
-        mlanguage.split_state σ1 pubσ privσ1 →
-        X (LkE (Expr1 e1) C, St1 σ1 privσ2)) →
-    prim_step_mrel p (LkE (RunFunction (inl fn1) args) C, σ) X
-  | RunFunction2S σ fn2 arg C X :
-    (∀ e2 σ2 pubσ privσ1 privσ2,
-        σ = St pubσ privσ1 privσ2 →
-        mlanguage.apply_func fn2 arg = Some e2 →
-        mlanguage.split_state σ2 pubσ privσ2 →
-        X (LkE (Expr2 e2) C, St2 privσ1 σ2)) →
-    prim_step_mrel p (LkE (RunFunction (inr fn2) arg) C, σ) X
-
-  (* Continuing execution by returning a value to its caller *)
-  | Ret1S v k1 σ C X :
-    (* Merging states is angelic/unique (see above) *)
-    (∀ pubσ privσ1 privσ2 σ1,
-          σ = St pubσ privσ1 privσ2 →
-          mlanguage.split_state σ1 pubσ privσ1 →
-          X (LkE (Expr1 (mlanguage.resume_with k1 (mlanguage.of_val Λ1 v))) C, St1 σ1 privσ2)) →
-    prim_step_mrel p (LkE (ExprV v) (inl k1::C), σ) X
-  | Ret2S v k2 σ C X :
-    (∀ σ2 pubσ privσ1 privσ2,
-          σ = St pubσ privσ1 privσ2 →
-          mlanguage.split_state σ2 pubσ privσ2 →
-          X (LkE (Expr2 (mlanguage.resume_with k2 (mlanguage.of_val Λ2 v))) C, St2 privσ1 σ2)) →
-    prim_step_mrel p (LkE (ExprV v) (inr k2::C), σ) X
+  (* Internal step of an underlying module. *)
+  | Step1S e1 C σ1 privσ2 (X1 X : _ → Prop) :
+    mlanguage.to_val e1 = None →
+    mlanguage.prim_step (proj1_prog p) (e1, σ1) X1 →
+    (∀ e1' σ1',
+      X1 (e1', σ1') →
+      X (LkE (Expr1 e1') C, St1 σ1' privσ2)) →
+    prim_step_mrel p (LkE (Expr1 e1) C, St1 σ1 privσ2) X
+  | Step2S e2 C σ2 privσ1 (X2 X : _ → Prop) :
+    mlanguage.to_val e2 = None →
+    mlanguage.prim_step (proj2_prog p) (e2, σ2) X2 →
+    (∀ e2' σ2',
+       X2 (e2', σ2') →
+       X (LkE (Expr2 e2') C, St2 privσ1 σ2')) →
+    prim_step_mrel p (LkE (Expr2 e2) C, St2 privσ1 σ2) X
   (* Stuck module calls bubble up as calls at the level of the linking module.
      (They may get unstuck then, if they match a function implemented by the
      other module.) *)
-
+  | MakeCall1S e1 C σ1 pubσ privσ1 privσ2 fn_name arg k1 X :
+    mlanguage.is_call e1 fn_name arg k1 →
+    proj1_prog p !! fn_name = None →
+    mlanguage.split_state σ1 pubσ privσ1 →
+    X (LkE (ExprCall fn_name arg) (inl k1 :: C), St pubσ privσ1 privσ2) →
+    prim_step_mrel p (LkE (Expr1 e1) C, St1 σ1 privσ2) X
+  | MakeCall2S e2 C σ2 pubσ privσ1 privσ2 fn_name arg k2 X :
+    mlanguage.is_call e2 fn_name arg k2 →
+    proj2_prog p !! fn_name = None →
+    mlanguage.split_state σ2 pubσ privσ2 →
+    X (LkE (ExprCall fn_name arg) (inr k2 :: C), St pubσ privσ1 privσ2) →
+    prim_step_mrel p (LkE (Expr2 e2) C, St2 privσ1 σ2) X
+  (* Producing a value when execution is finished *)
+  | Val1S e1 C σ1 v pubσ privσ1 privσ2 X :
+    mlanguage.to_val e1 = Some v →
+    (* Splitting the state is angelic, the underlying language can choose a concrete splitting. *)
+    (* If no such splitting exists, we have UB *)
+    mlanguage.split_state σ1 pubσ privσ1 →
+    X (LkE (ExprV v) C, St pubσ privσ1 privσ2) →
+    prim_step_mrel p (LkE (Expr1 e1) C, St1 σ1 privσ2) X
+  | Val2S e2 C σ2 v pubσ privσ1 privσ2 X :
+    mlanguage.to_val e2 = Some v →
+    (* Splitting the state is angelic, the underlying language can choose a concrete splitting. *)
+    (* If no such splitting exists, we have UB *)
+    mlanguage.split_state σ2 pubσ privσ2 →
+    X (LkE (ExprV v) C, St pubσ privσ1 privσ2) →
+    prim_step_mrel p (LkE (Expr2 e2) C, St2 privσ1 σ2) X
+  (* Entering a function. Change the view of the heap in the process.
+     Merging the state is angelic. *)
+  | RunFunction1S fn1 args C e1 σ1 pubσ privσ1 privσ2 X :
+    mlanguage.apply_func fn1 args = Some e1 →
+    mlanguage.split_state σ1 pubσ privσ1 →
+    X (LkE (Expr1 e1) C, St1 σ1 privσ2) →
+    prim_step_mrel p (LkE (RunFunction (inl fn1) args) C, St pubσ privσ1 privσ2) X
+  | RunFunction2S fn2 args C e2 σ2 pubσ privσ1 privσ2 X :
+    mlanguage.apply_func fn2 args = Some e2 →
+    mlanguage.split_state σ2 pubσ privσ2 →
+    X (LkE (Expr2 e2) C, St2 privσ1 σ2) →
+    prim_step_mrel p (LkE (RunFunction (inr fn2) args) C, St pubσ privσ1 privσ2) X
+  (* Continuing execution by returning a value to its caller. *)
+  | Ret1S v k1 C σ1 pubσ privσ1 privσ2 X :
+    mlanguage.split_state σ1 pubσ privσ1 →
+    X (LkE (Expr1 (mlanguage.resume_with k1 (mlanguage.of_val Λ1 v))) C, St1 σ1 privσ2) →
+    prim_step_mrel p (LkE (ExprV v) (inl k1 :: C), St pubσ privσ1 privσ2) X
+  | Ret2S v k2 C σ2 pubσ privσ1 privσ2 X :
+    mlanguage.split_state σ2 pubσ privσ2 →
+    X (LkE (Expr2 (mlanguage.resume_with k2 (mlanguage.of_val Λ2 v))) C, St2 privσ1 σ2) →
+    prim_step_mrel p (LkE (ExprV v) (inr k2 :: C), St pubσ privσ1 privσ2) X
   (* Resolve an internal call to a module function *)
-  | CallS fn_name arg σ C X :
-    (* Again, stuck calls cause UB *)
-    (∀ fn, p !! fn_name = Some fn →
-           X (LkE (RunFunction fn arg) C, σ)) →
-    prim_step_mrel p (LkE (ExprCall fn_name arg) C, σ) X.
+  | CallS fn_name fn arg σ C X :
+    p !! fn_name = Some fn →
+    X (LkE (RunFunction fn arg) C, σ) →
+    prim_step_mrel p (LkE (ExprCall fn_name arg) C, σ) X
+  (* Terminate execution with NB on values *)
+  | ValStopS v σ X :
+    prim_step_mrel p (LkE (ExprV v) [], σ) X.
 
   Program Definition prim_step (p : prog) : umrel (expr * state) :=
     {| mrel := prim_step_mrel p |}.
   Next Obligation.
     intros p. intros [[se k] σ] X Y Hstep HXY. inversion Hstep; subst;
-      [ eapply Step1S | eapply Step2S | eapply RunFunction1S | eapply RunFunction2S
-      | eapply Ret1S | eapply Ret2S | eapply CallS ]; eauto; naive_solver.
+      [ eapply Step1S | eapply Step2S | eapply MakeCall1S | eapply MakeCall2S
+      | eapply Val1S | eapply Val2S | eapply RunFunction1S | eapply RunFunction2S
+      | eapply Ret1S | eapply Ret2S | eapply CallS | eapply ValStopS ];
+      eauto; naive_solver.
   Qed.
 
   Lemma mlanguage_mixin :
@@ -205,33 +171,35 @@ Section Linking.
     constructor.
     - intros v. done.
     - intros e c. destruct e as [e [|]]; destruct e; cbn; intros; by simplify_eq.
-    - intros p v σ X. unfold of_val. inversion 1.
+    - intros *. eapply ValStopS.
     - intros p e fn_name arg C σ X ->. split.
-      + cbn. inversion 1; simplify_eq. intros fn' e H4' H5'.
-        unfold apply_func in H5'. simplify_eq. apply H5. done.
-      + intros H. cbn. unfold apply_func in H. econstructor. intros fn Heq.
-        eapply (H _ _ Heq eq_refl).
+      + inversion 1; simplify_eq. do 2 eexists. repeat split; eauto.
+      + intros (?&[]&?&?&?). unfold apply_func in *. simplify_eq.
+        econstructor; eauto.
     - intros e [v Hv] f vs C ->. done.
     - intros ? C1 C2 s vv ->. cbn. done.
-    - intros [se ec] C1 C2 s vv Hv Hc. rewrite /is_call /resume_with in Hc.
-      simplify_eq. eexists; repeat split; done.
     - intros [] C [v Hv]; cbn in Hv. repeat case_match; simplify_eq.
       apply app_eq_nil in H0 as [-> ->]. done.
     - intros [] C1 C2. rewrite /= app_assoc //.
-    - intros e s1 s2 f1 f2 C1 C2 -> H; unfold is_call in H; simplify_eq. done.
-    - intros p C [es eC] σ X Hnv H; inversion H; simplify_eq.
-      1-2: econstructor; by eauto. (* Step*S *)
-      1-2: econstructor; by eauto. (* RunFunctionS *)
-      1-2: destruct eC; simplify_list_eq; []; econstructor; by eauto. (* RetS *)
-      1: econstructor; eauto.
-    - intros p [[] eC] σ Hnv; simplify_eq.
-      + destruct eC as [|[] eC']; first done. all: by econstructor.
-      + by econstructor.
-      + destruct fn; by econstructor.
-      + econstructor; eauto. intros. exists (λ _, True). split; eauto.
-        by eapply prim_step_is_total.
-      + econstructor; eauto. intros. exists (λ _, True). split; eauto.
-        by eapply prim_step_is_total.
+    - intros p C [es eC] σ X Hnv. inversion 1; simplify_eq.
+      1,2: econstructor; eauto; intros; eexists (LkE _ _); by eauto. (* StepS *)
+      { eapply MakeCall1S; eauto; eexists (LkE _ _); split; eauto;
+          unfold resume_with; by eauto. }
+      { eapply MakeCall2S; eauto; eexists (LkE _ _); split; eauto;
+          unfold resume_with; by eauto. }
+      { eapply Val1S; eauto. eexists (LkE _ _). split; eauto. }
+      { eapply Val2S; eauto. eexists (LkE _ _). split; eauto. }
+      1,2: econstructor; eauto; eexists (LkE _ _); split; eauto. (* RunFunctionS *)
+      1,2: econstructor; eauto; eexists (LkE _ _); split; eauto. (* RetS *)
+      eapply CallS; eauto; eexists (LkE _ _); split; eauto.
+    - intros p [[] eC] σ Hnv; simplify_eq;
+        try by (intros _; inversion 1; simplify_eq; eauto).
+      + destruct eC as [|[] eC']; first done; intros _;
+          inversion 1; simplify_eq; eauto.
+      + intros _. inversion 1; simplify_eq; eauto.
+        eapply prim_step_no_NB in H5 as (e1 & σ1' & ?); eauto.
+      + intros _. inversion 1; simplify_eq; eauto.
+        eapply prim_step_no_NB in H5 as (e2 & σ2' & ?); eauto.
   Qed.
 End Linking.
 End Link.
