theories/mlanguage/lifting.v
@@ -17,19 +17,19 @@ Implicit Types Φ : val → iProp Σ.
 Implicit Types X : expr Λ * state Λ → Prop.
 
 Lemma wp_lift_step_fupd pe E Φ e1 :
-  to_val e1 = None → 
+  to_val e1 = None →
   not_is_ext_call (penv_prog pe) e1 →
   (∀ σ1, state_interp σ1 ={E}=∗
-    ∀ X, ⌜prim_step (penv_prog pe) (e1, σ1) X⌝ ={E}▷=∗^(1) |={E}=>
-      ∃ e2 σ2,
-        ⌜X (e2, σ2)⌝ ∗ state_interp σ2 ∗ WP e2 @ pe; E {{ Φ }})
+    ∃ X, ⌜prim_step (penv_prog pe) (e1, σ1) X⌝ ∗ |={E}▷=>
+      ∀ e2 σ2,
+        ⌜X (e2, σ2)⌝ -∗ state_interp σ2 ∗ WP e2 @ pe; E {{ Φ }})
   ⊢ WP e1 @ pe; E {{ Φ }}.
 Proof. intros Hval Hcall. rewrite wp_unfold /wp_pre.
-  iIntros "H %σ Hσ". iMod ("H" $! σ with "Hσ") as "H2". iModIntro. do 2 iRight.
+  iIntros "H %σ Hσ". iMod ("H" $! σ with "Hσ") as (? ?) "H2". iModIntro. do 2 iRight.
+  iSplitR; first done. iExists _.
   iSplitR; first done.
-  iSplitR; first done.
-  iIntros (X Hstep). iMod ("H2" $! X Hstep) as "H2". do 2 iModIntro.
-  do 2 iMod "H2". iModIntro. iFrame.
+  iIntros (? ? HX). iMod "H2". do 2 iModIntro. iMod "H2".
+  iModIntro. iSpecialize ("H2" $! _ _ HX). iFrame.
 Qed.
 
 
@@ -40,56 +40,34 @@ Lemma wp_lift_atomic_step {pe E Φ} e1 :
   to_val e1 = None →
   not_is_ext_call (penv_prog pe) e1 →
   (∀ σ1, state_interp σ1 ={E}=∗
-    ▷ ∀ X, ⌜prim_step (penv_prog pe) (e1, σ1) X⌝ ={E}=∗
-      ∃ e2 σ2, ⌜X (e2, σ2)⌝ ∗
+    ∃ X, ⌜prim_step (penv_prog pe) (e1, σ1) X⌝ ∗ |={E}▷=>
+      ∀ e2 σ2, ⌜X (e2, σ2)⌝ -∗
         state_interp σ2 ∗ from_option Φ False (to_val e2))
   ⊢ WP e1 @ pe; E {{ Φ }}.
 Proof.
   iIntros (Hnv Hnc) "H".
   iApply (wp_lift_step_fupd pe E _ e1)=>//; iIntros (σ1) "Hσ1".
-  iMod ("H" $! σ1 with "Hσ1") as "H". iModIntro.
-  iIntros (X Hstep). do 3 iModIntro.
-  iMod ("H" $! X Hstep) as (e' σ' HX) "[? ?]". iModIntro.
-  iExists _, _. iSplitR; first done. iFrame.
-  destruct (to_val e') eqn:?; last by iExFalso.
-  by iApply wp_value.
-Qed.
-
-Lemma wp_lift_atomic_prim_step {pe E Φ} e1 :
-  to_val e1 = None →
-  not_is_ext_call (penv_prog pe) e1 →
-  (∀ σ1, state_interp σ1 ={E}=∗
-    ▷ ∀ X, ⌜prim_step (penv_prog pe) (e1, σ1) X⌝ ={E}=∗
-      ∃ e2 σ2, ⌜X (e2, σ2)⌝ ∗
-        state_interp σ2 ∗ from_option Φ False (to_val e2))
-  ⊢ WP e1 @ pe; E {{ Φ }}.
-Proof.
-  iIntros (Hnv Hnc) "H".
-  iApply (wp_lift_step_fupd pe E _ e1)=>//; iIntros (σ1) "Hσ1".
-  iMod ("H" $! σ1 with "Hσ1") as "H". iModIntro.
-  iIntros (X Hstep).
-  do 3 iModIntro. iMod ("H" $! X Hstep) as "(%e2&%σ2&%HX&Hσ&H)".
-  iExists _, _. iSplitR; first done. iModIntro. iFrame.
+  iMod ("H" $! σ1 with "Hσ1") as (X Hstep) ">H". iModIntro.
+  iExists _. iSplit; first done. do 2 iModIntro.
+  iMod "H". iIntros "!>" (? ? HX).
+  iDestruct ("H" $! _ _ HX) as "[? ?]". iFrame.
   destruct (to_val e2) eqn:?; last by iExFalso.
   by iApply wp_value.
 Qed.
 
 Lemma wp_lift_pure_det_step `{!Inhabited (state Λ)} {pe E Φ} e1 e2 :
   (to_val e1 = None) →
-  (∀ σ1 X,
-    prim_step (penv_prog pe) (e1, σ1) X →
-    X (e2, σ1)) →
+  (∀ σ1, prim_step (penv_prog pe) (e1, σ1) (λ '(e', σ'), e' = e2 ∧ σ' = σ1)) →
   (|={E}[E]▷=> WP e2 @ pe; E {{ Φ }}) ⊢ WP e1 @ pe; E {{ Φ }}.
 Proof.
   iIntros (Hsafe Hstep) "H". iApply wp_lift_step_fupd; first done.
-  { intros (f&vs&C&H1&H2). eapply (Hstep inhabitant (λ _, False)).
-    eapply call_prim_step; first done.
-    intros ? ? ?; congruence. }
+  { intros (f&vs&C&H1&H2). specialize (Hstep inhabitant).
+    eapply call_prim_step in Hstep as (?&?&?&?&?&?); eauto.
+    simplify_eq. }
   iIntros (σ1) "Hσ". iMod "H". iModIntro.
-  iIntros (X Hstep'). do 3 iModIntro. iMod "H".
-  iModIntro. iExists e2, _. iSplitR.
-  { iPureIntro. eapply Hstep; eauto. }
-  iFrame.
+  iExists _. iSplit; first done.
+  do 2 iModIntro. iMod "H".
+  iModIntro. iIntros (? ? (-> & ->)). iFrame.
 Qed.
 
 End lifting.
